Engine/Meta/Meta.v
@@ -49,7 +49,7 @@ Definition meta_search_anchored (config:meta_config) (r:regex) (inp:input) : opt
     (* FIXME: how come we do not need to provide the MemoSet instance? *)
     @exec _ _ (@MemoBTAnchoredEngine _ rer) r inp
   else
-    @exec _ _ (@PikeVMAnchoredEngine VMSlist _ rer BruteForceStrSearch) r inp.
+    @exec _ _ (@PikeVMAnchoredEngine VMSlist _ rer) r inp.
 
 Theorem meta_search_anchored_correct (config:meta_config):
   forall r inp tree,
